#### 1 (a) 
A derivation on p20 of the handout gives
\begin{equation*}
  \label{eq:fib}
  \sum_{n=0}^{\infty}f_nx^n = \frac{x}{1-x-x^2}
\end{equation*}
By differentiating both sides, 
\begin{align}
  \label{eq:fibdiff}
  \sum_{n=0}^{\infty}nf_nx^{n-1} &= \frac{(1-x-x^2) - x(-1-2x)}{(1-x-x^2)^2}\\
  &= \frac{1 + x^2}{(1-x-x^2)^2}.
\end{align}
By substituting $1/2$ for $x$, 
\begin{align*}
  \sum_{n=0}^{\infty}\frac{nf_n}{2^{n-1}}
  = \frac{1 + \frac{1}{4}}{(1-\frac{1}{2}-\frac{1}{4})^2}
  = \frac{\frac{5}{4}}{\frac{1}{16}}
    = 20.
\end{align*}

#### 1 (b)
Substituting $1$ for $x$ in (\ref{eq:fibdiff}) would appear to give
\begin{align}
  \label{eq:fibdiffconscrazy}
  \sum_{n=0}^{\infty}nf_n = \frac{(1-1-1) - 1(-1-2)}{(1-1-1)^2} = 2.
\end{align}
However, (\ref{eq:fibdiffconscrazy}) is false; indeed, the sum on the left hand side does not converge at all.  For, toward a contradiction, suppose that the sum converges to $d$.  Since $f_n>n$  for all $n>3$ (as is clear by induction on $n$), it follows that $nf_n>n$ for all $n>3$.  Thus,  $\sum_{n=0}^{e}nf_n > d+1$ for any $e$ greater than both $d$ and $3$.  So, any partial sum of length at least $e$ cannot come within even $\epsilon=1$ of $d$, contradicting the definition of convergence.

#### 2(a)
 According to the binomial theorem,
\begin{equation}
  \label{eq:binthm}
  (1+x)^n = \sum_{k=0}^{n}\binom{n}{k}x^k.
\end{equation}

#### 2(b)
 Similarly,
\begin{equation}
  \label{eq:binthm2}
  (1-x)^n = \sum_{k=0}^{n}\binom{n}{k}(-x)^k.
\end{equation}

#### 2(c)
 Using (\ref{eq:binthm}) and (\ref{eq:binthm2}) above,
\begin{align*}
  (1 + x)^n + (1 - x)^n
  &= \sum_{k=0}^{n}\binom{n}{k}x^k + \sum_{k=0}^{n}\binom{n}{k}(-x)^k\\
  &= \sum_{k=0}^{n}\binom{n}{k}(x^k + (-x)^k)\\
  &= 2(\binom{n}{0}x^0 + \binom{n}{2}x^2 + \binom{n}{4}x^4 + \cdots).
\end{align*}

#### 2(d)
 Likewise using (\ref{eq:binthm}) and (\ref{eq:binthm2}) above,
\begin{align}
\label{eq:bincons}
  \nonumber (1 + x)^n - (1 - x)^n
  &= \sum_{k=0}^{n}\binom{n}{k}x^k - \sum_{k=0}^{n}\binom{n}{k}(-x)^k\\
  \nonumber
  &= \sum_{k=0}^{n}\binom{n}{k}(x^k - (-x)^k)\\
  &= 2(\binom{n}{1}x^1 + \binom{n}{3}x^3 + \binom{n}{5}x^5 + \cdots).
\end{align}

#### 2(e)
 Setting $x=1$, the equation (\ref{eq:bincons}) implies
\begin{equation*}
  2^n = (1 + 1)^n - (1 - 1)^n = 2(\binom{n}{1} + \binom{n}{3} + \binom{n}{5} + \cdots)
\end{equation*}
and so
\begin{equation*}
   \binom{n}{1} + \binom{n}{3} + \binom{n}{5} + \cdots = 2^{n-1}
\end{equation*}
which should be simple enough for the econ prof!

#### 3 (a)
Let me write $f(n) = n^2$ and $g(n) = 2^n$. 
Now, note that
\begin{equation*}
f(n+1) = (n+1)^2 = n^2 + 2n + 1 = f(n) + 2n + 1  
\end{equation*}
while
\begin{equation*}
g(n+1)=2^{n+1}=g(n)+g(n).
\end{equation*}
It follows that if $g(n)>f(n)$ and $g(n)>2n+1$, then $g(n+1)>f(n+1)$.

I'll argue that $g(n) > 2n+1$ for all $n\geq 5$.  This is clear for $n=5$.  Now assume that $g(n)>2n+1$.  Then
\begin{equation*}
g(n+1) = 2*g(n) > 2(2n + 1) > 2(n+1) + 1  
\end{equation*}
and so the claim follows by induction.

The above two claims imply that if $g(n)>f(n)$, then $g(n+1)>f(n+1)$ for all $n>4$.  However, $g(5)>f(5)$.  So if $x=5$, then $f(n)\leq g(n)$ for all $n\geq x$.  So $f\in O(g)$, as desired.

#### 3 (b)
 Note that $2^{n+1} = 2*(2^n)$.  So if $c=2$ and $x=0$, it follows that that $2^{n+1}\leq c*2^n$ for all $n\geq x$.

#### 3 (c)
 Suppose there were $c,x$ such that $2^{2n} \leq  c*2^n$ for all $n>=x$.
Since $2^n>0$, it follows from $2^{2(n+1)} \leq  c * 2^{n+1}$
that $2^{n+1} \leq  c$ for all $n>=x$.  

However, $2^n>n$ for all $n>=0$ (as is readily proved by induction on $n$).  Hence,
$2^{c+1}> c+1 > c$.  We must therefore have $c<x$, so that $c < x < 2^x < 2^{x+1}$, a contradiction.

#### 3 (d)
Let $f(n) = 2n$, and let $g(n) = n$.  Clearly $f\in O(g)$, since we may pick $c=2$.  But, writing $\hat f(n) = 2^{f(n)}$ and $\hat g(n) = 2^{g(n)}$, the above response to exercise 3c says precisely that $\hat f\not\in O(\hat g)$.

#### 4
  First, note that $a^{\log_a(x)} = x$, so that 
\begin{equation}
  \log_a(x) * \log_b(a) = \log_b(a^{\log_a(x)})  = \log_b(x).
\end{equation}
Therefore
\begin{equation}
  \log_a(x) = \log_b(x)/\log_b(a)
\end{equation}
 (the ``change of base formula'').  So setting $c=1/\log_b(a)$ and $x=1$, it follows that $\log_a(x_0)\leq c*log_b(x_0)$ for all $x_0>x$.

#### 5 (a)
 I'll argue by induction on $n$.  Clearly $x^{j}\in O(x^n)$ if $n=j$.  Now, suppose that $x^j \leq c*x^n$ for all $x$.  Picking $\hat x$ to be the greater of $x$ and $1$, it follows that $x^j \leq c*x^n \leq c *x^{n+1}$ for all $x\geq \hat x$, as desired.

Before continuing to (b), note that if $g\in O(f)$, then $O(g)\subseteq O(f)$.  Hence part (a) implies that $O(x^j)\subseteq O(x^n)$ for all $j\leq n$.

#### (b) 
I'll argue by induction on $n$. The claim is trivial for $n=1$.  Writing $p(x) = \sum_{i=1}^{n}a_nx^n$, suppose that $\sum_{i=1}^{n}a_nx^n \in O(x^n)$.  It then follows from the above remark on part (a) that $p(x) \in O(x^{n+1})$.  Meanwhile, clearly $a_{n+1}x^{n+1} \in O(x^{n+1})$.  The claim follows from the fact that $O(x^{n+1})$ is closed under addition (Lemma 3.1 in the handout).

It now suffices to show that $O(f)$ is closed under addition for any $f$.  Well if $O(f)$ contains both $g$ and $h$, then there are $x_0, x_1$ and $c_0, c_1$ such that $g(n)\leq c_0*f(n)$ and $h(n)\leq c_1*f(n)$ for all $n$ respectively no less than $x_0, x_1$.  Picking $c$ and $x$ as $c_0+c_1$ and the larger of $x_0, x_1$, it follows that $g(x) + h(x) \leq c*f(n)$ for all $n \geq x$.

#### (c)
First, note that $p(x)>= a_nx^{n}$ for all $x>0$, so it suffices to show that $a_nx^{n}\in \Omega(x^n)$.  Since $a_n>0$, we may simply pick $c=a_n$ to affirm that $a_nx^n >= cx^n$ for all $x$ so that $a_nx^n\in \Omega(x^n)$ as desired.

#### (d)
Suppose that $p(x)\in O(x^d)$, where $p(x) = \sum_{i=1}^na_ix^i$.  Toward a contradiction further suppose that $a_n>0$.  Then likewise $a_nx^n\in O(x^d)$, and so, since $a_n>0$, also $x^n\in O(x^d)$.  Then there are $c, \hat x$ such that $x^n \leq cx^d$ for all $x\geq\hat x$.  So writing $m=n-d$, we have $m>1$ while $x^m \leq c$ for all $x\geq \hat x$.  This contradicts the fact that $x^m > c$ for any $x$ greater than both $1$ and $c$.

#### 6
Suppose that $f\in O(g)$ and $g\in O(h)$.  Then there are $c_0,c_1,x_0, x_1$ such that $f(x)\leq c_0g(x)$ and $g(x)\leq c_1h(x)$ for all $x$ greater than $x_0,x_1$ respectively.  Picking $c$ to be $c_0c_1$ and $\hat x$ to be the larger of $x_0,x_1$, it follows that $f(x)\leq ch(x)$ for all $x\geq \hat x$.

#### 7 (a)
$T(n) = 2T(\frac{n}{2}) + n^4$. Setting $a=2$ and $b=2$, it follows that $\log_b a = 1$ so that $f(n) = n^4\in O(n^{\log_b a + \epsilon})$ for $\epsilon=3$.  Furthermore, picking $c=1$,
\begin{equation*}
af(\frac{n}{b}) = 2(\frac{n}{2})^4 = \frac{n^4}{8}\leq n^4 = cf(n)  
\end{equation*}
for all sufficiently large $n$ (e.g., $>1$).

So, we are in case (3) of the master theorem, and $T(n) = \Theta(f(n)) = \Theta(n^4)$.

#### (b)
$T(n) = T(\frac{7n}{10}) + n$.  Setting $a=1$ and $b=\frac{10}{7}$, it follows that $\log_ba=\log_{\frac{10}{7}}1 = 0$.  So here $f(n) = n^1 \in O(n^{\log_b a + \epsilon})$ for $\epsilon = 1$.  Furthermore, again picking $c=1$, 
\begin{equation*}
  f(\frac{7n}{10})=\frac{7n}{10}\leq n = cf(n)
\end{equation*}
for all $n>=0$.

So we are again in case (3) of the master theorem, and $T(n) = \Theta(f(n))=\Theta(n)$.

#### (c)
$T(n) = 16T(\frac{n}{4}) + n^2$.  With $a=16, b=4$, it follows that $f(n)=n^2\in O(n^2)=O(n^{\log_b a})$.

Here we are in case (2) of the master theorem, and $T(n)=\Theta(n^{\log_b a}\lg n)=\Theta(n^2\lg n)$.

#### (f)
$T(n) = 2T(\frac{n}{4}) + \sqrt n$.  With $a=2, b=4$, it follows that $f(n)=\sqrt{n} = n^{\frac{1}{2}}\in O(n^{\frac{1}{2}})=O(n^{\log_b a})$.

So again we are in case (2) of the master theorem, and $T(n)=\Theta(n^{\log_b a}\lg n=\Theta(\sqrt{n}\lg n)$.

#### (g)
$T(n) = T(n-2) + n^2$.  In this case, the recurrence doesn't have a form suited to the master theorem.  However, note for example that
\begin{equation*}
T(7) = T(1) + 3^2 + 5^2 + 7^2,  
\end{equation*}
and this clearly generalizes: $T(n)$ is the sum of a constant plus the squares of all odd numbers from $3$ up to $n$.  Geometrically, the sum can be approximated as a pyramid with with base lengths and height each in some constant ratio to $n$.  So a reasonable guess is that $T(n) \in \Theta(n^3)$.

Following the substitution method, I'll now argue first, by induction on $n$, that 
$T(n)\geq \frac{1}{6}n^3$ for all $n\geq 3$.  For the basis step, we need to consider both $n=3$ and $n=4$, which amounts to observing that $3^2+T(1) \geq \frac{1}{6}3^3$ and that $4^2+T(1) \geq \frac{1}{6}4^3$.  Assuming now that $T(m)\geq \frac{1}{6}m^3$ for all $m<n$, it follows for $n>4$ that
\begin{align*}
  T(n) &= T(n - 2) + n^2\\
       &\geq \frac{1}{6}(n-2)^3 + n^2\\
       &= \frac{1}{6}(n^3 - 6n^2 + 12n - 8) + n^2\\
       &= \frac{1}{6}n^3 + 2n - \frac{4}{3}\\
       &\geq \frac{1}{6}n^3.
\end{align*}
It remains to find conversely an bound on $T$.  For simplicity, let's assume that the times $T(1)$ and $T(2)$ are negligible (since $T$ is clearly unbounded, it will eventually swamp whatever constants they may be).  I'll argue, again by induction on $n$, that $T(n)\leq n^3$ for all $n\geq 12$.  It's easy to verify that this holds for $n=12$ and $n=13$, so suppose that it holds for all $m<n$.  It follows, certainly for $n>13$, that \begin{align*}
  T(n) &= T(n - 2) + n^2\\
       &\leq n^3 - 6n^2 + 12n - 8 + n^2\\
       &= n^3 -5n^2 +12n - 8\\
       &\leq n^3.
\end{align*}

#### 8.
[See attachment.]

#### 9 (a)
There exist nonempty sets of points in the plane such there is no uniquely closest pair.  For example, $\{(0,1),(0,2),(0,3)\}$.

#### (b)
The algorithm takes time proportional to $n^2$, for all $n$.  To see this, note that the collection of pairs of elements of an $n$-element set has size proportional to $n^2$.  (If the pairs are ordered pairs, it is exactly $n^2$, else it is $\frac{n(n+1)}{2}$).  Since the algorithm measures a distance for each pair, it must take at least $\sim n^2$ steps.  Conversely, it requires only a constant number of tasks per pair; besides measuring the distance $d$, it must compare $d$ with the current maximum distance $m$ and in the worst case replace $m$ with $d$.

#### 10.
Suppose that the nodes of a binary tree are decorated with the entry of an array $A$.  Specifically, the node of depth $0$ is decorated with the first entry $A[0]$, the nodes at depth $1$ with the second and third entries $A[1]$ and $A[2]$, and so on.  I will assume that the entries of the array are all distinct, and therefore instead simply say that a given node has numerical index $i$ when it is decorated by $A[i]$.  Now, here is the claim to be proven:
\begin{itemize}
\item[(A)] If a given node $N$ has index $n$, then its children have indices $2n$ and $2n+1$.
\end{itemize}

To verify the claim, first note two facts (here and throughout, I assume each row under consideration is ``completely filled out''):
\begin{itemize}
\item[(B)] The number of nodes of depth $d$ is $2^d$.  This is clear for $d=0$.  As for $d+1$, by induction there are $2^d$ nodes of depth $d$, and the nodes of depth $d+1$ are precisely the children of a node of depth $d$.  Also, each node has two children, and no two nodes have a child in common.  So, there are $2*d^2=d^{2+1}$ nodes of depth $d$.
\item[(C)] The number of all nodes of depth less than $d$ is $2^d$.  This is vacuously true for $d=0$.  Now, note that the nodes of depth less than $d$ are precisely the nodes of depth less than $d-1$, together with the nodes of depth $d-1$ itself.  So supposing the number of nodes of depth less than $d-1$ to be $2^{d-1}$, it follows by fact (A) that the number of nodes of depth $d$ is $2^{d-1}+2^{d-1}=2^d$.
\end{itemize}
From facts (B) and (C), it is immediate that the $i$th node of depth $d$ has index  $2^d+i$.  Moreover, the $i$th node at a given depth has precisely $i$ predecessors at that depth (I am assuming $0$-indexing, per the problem statement).  So, the children of the $i$th node at $d$ have $2i$ and $2i+1$ predecessors at depth $d+1$.  Thus, the children have indices $2^{d+1}+2i$ and $2^{d+1}+2i+1$ respectively.  However, $2^{d+1}+2i = 2(2^{d}+i)$.  It follows (writing $n=2^d+i$, as is always possible) that the children of the node with index $n$ have indices $2n$ and $2n+1$, as desired.





